Handout 2/handout2_task3.dfy
@@ -1,0 +1,223 @@
+/**
+CVS 2021-22 Handout 2 - Task 1
+Authors
+Gonçalo Martins Lourenço nº55780
+Joana Soares Faria  nº55754
+ */
+
+class IntervalTree {
+
+    //The actual tree 
+    var tree: array<int>
+
+    /*The number of leaves in the tree (i.e. the number of elements in the sequence). */ 
+    ghost var leaves: int
+
+    ghost var s : seq<int> // for task tree
+
+    predicate ValidSize() 
+        reads `tree, `leaves
+    {
+        tree.Length == 2*leaves-1 
+    }
+
+    predicate Valid() 
+        reads this, `tree, `leaves, tree
+    {
+        ValidSize() 
+        && 
+        forall i :: 0 <= i < leaves - 1 ==> tree[i] == tree[2*i+1] + tree[2*i+2]
+        && |s| == leaves 
+        && tree[0] == sum(s)
+        && forall i:: 0 <= i < leaves ==> s[i] == get(i)
+    }
+
+    /*Initializes an interval tree for a sequence of n elements whose values are 0. */ 
+    constructor(n: int) 
+        requires n > 0 
+        ensures leaves == n 
+        ensures Valid()
+        ensures forall i :: 0 <= i < n ==> get(i) == 0
+        ensures fresh(tree)
+    {
+        tree := new int[2 * n - 1] (i => 0); 
+        leaves := n;
+
+        var i := 0;
+        s := s + [0];
+
+        while(i < n) 
+            decreases n-i
+            // invariant forall j :: 0 <= j < i ==> s[j] == get(j)
+        {
+            i:=i+1;
+            s := s + [0];
+            
+        }
+    }
+
+    //Updates the i-th sequence element (0-based) by v 
+    method update(i: int,v: int) 
+        modifies tree
+        requires 0 <= i < leaves
+        requires Valid()
+        ensures forall j:: 0 <= j < leaves ==> if (j != i) 
+                                            then get(j) == old(get(j)) 
+                                            else get(j) == old(get(j)) + v
+        ensures Valid() 
+    {
+        var pos := tree.Length/2 + i; 
+        tree[pos] := tree[pos] + v;
+        
+        // assert pos == i + leaves - 1;
+        
+        while(pos > 0) 
+            decreases pos 
+            invariant 0 <= pos <= tree.Length/2 + i
+            invariant forall j:: 0 <= j < leaves ==> if (j != i) 
+                                        then get(j) == old(get(j)) 
+                                        else get(j) == old(get(j)) + v       
+            invariant forall k:: 0 <= k <  tree.Length / 2 ==> if k == (pos - 1) / 2
+                                                    then tree[k] == tree[2*k+1] + tree[2*k+2] - v 
+                                                    else tree[k] == tree[2*k+1] + tree[2*k+2]
+            //invariant forall k:: 0 <= k <  tree.Length / 2 ==> tree[k] == tree[2*k+1] + tree[2*k+2] - if (k == (pos - 1) / 2) then v else 0 
+        {
+            pos := (pos-1)/2;  
+            tree[pos] := tree[pos] + v; 
+        }
+
+    }
+
+    //Ranged sum over interval [a,b[ 
+    method query(a: int, b: int) returns (r: int) 
+        requires 0 <= a <= b <= leaves
+        requires Valid()
+        ensures r == rsum(a,b) 
+        ensures Valid()
+    {
+    
+        var ra := tree.Length/2 + a;
+        var rb := tree.Length/2 + b;
+        r := 0;
+        
+        shift(a, b, leaves-1);
+       
+        while(ra < rb)
+            invariant 0 <= ra <= tree.Length/2 + a;
+            invariant 0 <= rb <= tree.Length/2 + b;
+            invariant r + sumArr(ra,rb) == rsum(a,b)
+            decreases ra, rb;
+        {
+            sumArrSwap(ra,rb);
+        
+            //If ra is rigth child we add the array value
+            if(ra % 2 == 0) {
+                r := r + tree[ra];
+            }
+            //move up to ra parent
+            ra := ra/2;
+
+            // if rb is a right-child, since the interval is open on its upper-bound, we must include the value at position rb-1 in our sum because its node must be a leftchild.
+            if(rb % 2 == 0) {
+                r := r + tree[rb-1];
+            }
+
+            //move up to rb parent
+            rb := (rb-1)/2;
+
+            crucial(ra, rb);
+
+        }
+    }
+    
+    /*ith element of the sequence, through the array-based representation*/ 
+    function get(i: int) : int 
+        requires 0 <= i < leaves && ValidSize() 
+        reads tree, `leaves, `tree
+    {
+        tree[i+leaves-1]
+    }
+
+    //Sum of elements over range [a,b[ 
+    function rsum(a: int,b: int) : int 
+        requires Valid() 
+        decreases b-a 
+        requires 0 <= a <= leaves && 0 <= b <= leaves 
+        reads this, `tree, `leaves, tree
+    {
+        if b <= a then 0 else get(b-1) + rsum(a, b-1) 
+    }
+
+    function sumArr(a: int,b: int) : int 
+        requires Valid() 
+        requires 0 <= a <= tree.Length && 0 <= b <= tree.Length 
+        reads this, `tree, `leaves, tree
+    {
+        if b <= a then 0 else tree[b-1] + sumArr(a,b-1) 
+    }
+
+    lemma shift(a: int,b: int,c: int) 
+        requires Valid() && 0 <= c <= leaves-1 
+        requires 0 <= a <= leaves && 0 <= b <= leaves 
+        requires forall i:: a <= i < b ==> get(i) == tree[i+c] 
+        // requires ∀ i • a ≤ i < b =⇒ get(i) = tree[i+c] 
+        ensures rsum(a,b) == sumArr(a + c, b + c) 
+        decreases b-a
+    {
+        if(b > a) {
+            shift(a,b-1, c);
+        }
+    }
+
+    lemma crucial(ra: int,rb: int) 
+        requires 0 <= ra <= rb && 2*rb < tree.Length && Valid() 
+        ensures sumArr(ra,rb) == sumArr(2*ra+1,2*rb+1)
+    {
+        if(ra < rb){
+            crucial(ra, rb-1);
+        }
+
+    }
+
+    lemma sumArrSwap(ra: int,rb: int) 
+        requires Valid() 
+        requires 0 <= ra < rb && 0 <= rb <= tree.Length 
+        ensures sumArr(ra,rb) == tree[ra]+sumArr(ra+1,rb)
+    {
+         if(ra < rb-1){
+            sumArrSwap(ra, rb-1);
+        }
+    }
+
+
+    function sum(s: seq<int>) :int {
+       if |s| == 0 then 0 else s[0]+sum(s[1..])
+    }
+
+
+// TASK 3
+   lemma sum_zero(s: seq<int>) 
+    requires forall i:: 0 <= i < |s| ==> s[i] == 0 
+    ensures sum(s) == 0{
+       
+    }
+
+
+    lemma sum_elem(s: seq<int>,x: int,p: int) 
+    requires 0 <= p < |s| 
+    ensures x+sum(s) == sum(s[p := s[p]+x]){
+       
+    }
+
+}
+
+// method Main(){
+//     var t := new IntervalTree(10);
+//     var r := t.query(1, 3);
+//     t.update(1, 1);
+//     t.update(2, 1);
+//     var y := t.query(2, 3);
+//     // t.update(0, 1);
+
+
+// }
